src/arch/Types_i.fsti
@@ -62,7 +62,22 @@ val lemma_equality_check_helper (q:quad32) :
          (q.lo0 == 0xFFFFFFFF /\ q.lo1 == 0xFFFFFFFF <==> lo64 q == 0xFFFFFFFFFFFFFFFF) /\
          (q.hi2 == 0xFFFFFFFF /\ q.hi3 == 0xFFFFFFFF <==> hi64 q == 0xFFFFFFFFFFFFFFFF)
          )
-         
+
+let lemma_equality_check_helper_2 (q1 q2 cmp:quad32) (tmp1 result1 tmp2 tmp3 result2:nat64) : Lemma
+  (requires cmp == Mkfour (if q1.lo0 = q2.lo0 then 0xFFFFFFFF else 0)
+                          (if q1.lo1 = q2.lo1 then 0xFFFFFFFF else 0)
+                          (if q1.hi2 = q2.hi2 then 0xFFFFFFFF else 0)
+                          (if q1.hi3 = q2.hi3 then 0xFFFFFFFF else 0) /\
+            tmp1 = lo64 cmp /\
+            result1 = (if tmp1 = 0xFFFFFFFFFFFFFFFF then 0 else 1) /\
+            tmp2 = hi64 cmp /\
+            tmp3 = (if tmp2 = 0xFFFFFFFFFFFFFFFF then 0 else 1) /\
+            result2 = tmp3 + result1)
+  (ensures (if q1 = q2 then result2 = 0 else result2 > 0))
+  =
+  lemma_equality_check_helper cmp;
+  ()
+
 val push_pop_xmm (x y:quad32) : Lemma 
   (let x' = insert_nat64 (insert_nat64 y (hi64 x) 1) (lo64 x) 0 in
    x == x')
@@ -79,27 +94,12 @@ val le_quad32_to_bytes_to_quad32 (s:seq nat8 { length s == 16 }) :
 val le_seq_quad32_to_bytes_of_singleton (q:quad32) :
   Lemma (le_quad32_to_bytes q == le_seq_quad32_to_bytes (create 1 q))
 
-let le_quad32_to_bytes_injective ():
+val le_quad32_to_bytes_injective: unit ->
   Lemma (forall b b' . le_quad32_to_bytes b == le_quad32_to_bytes b' ==> b == b')
-  =
-  let helper (b b':quad32) : Lemma (le_quad32_to_bytes b == le_quad32_to_bytes b' ==> b == b') =
-    if le_quad32_to_bytes b = le_quad32_to_bytes b' then (
-      let b1  = seq_map (nat_to_four 8) (four_to_seq_LE b) in
-      let b1' = seq_map (nat_to_four 8) (four_to_seq_LE b') in
-      assert (le_quad32_to_bytes b == seq_four_to_seq_LE b1);
-      assert (le_quad32_to_bytes b' == seq_four_to_seq_LE b1');
-      seq_four_to_seq_LE_injective_specific b1 b1';
-      assert (b1 == b1');
-      seq_map_injective (nat_to_four 8);
-      nat_to_four_8_injective();
-      assert ((four_to_seq_LE b) == (four_to_seq_LE b'));
-      four_to_seq_LE_injective nat32;
-      ()
-    ) else
-    ()
-  in 
-  FStar.Classical.forall_intro_2 helper
-  
+
+val le_quad32_to_bytes_injective_specific (b b':quad32) : 
+  Lemma (le_quad32_to_bytes b == le_quad32_to_bytes b' ==> b == b')
+
 val seq_to_four_LE_is_seq_to_seq_four_LE (#a:Type) (s:seq4 a) : Lemma
   (create 1 (seq_to_four_LE s) == seq_to_seq_four_LE s)
 
